

❑ **Example 1:**  $F = \{ a \rightarrow b, b c \rightarrow d, a c \rightarrow d \}$

Give the minimal cover  $M$  for the set  $F$  of FDs.

❑ **Step 1:**  $F = \{ a \rightarrow b, b c \rightarrow d, a c \rightarrow d \}$

❑ **Step 2:**

1) 假设去掉  $a \rightarrow b$ , 则  $F = \{ b c \rightarrow d, a c \rightarrow d \}$

计算  $\{ a \}_F^+ = \{ a \}$

$\therefore b \notin \{ a \}_F^+$

$\therefore$  不能去掉  $a \rightarrow b$

- ❑ **Example 1:**  $F = \{ a \rightarrow b, b c \rightarrow d, a c \rightarrow d \}$   
Give the minimal cover  $M$  for the set  $F$  of FDs.

❑ **Step 2:**

2) 假设去掉  $b c \rightarrow d$ , 则  $F = \{ a \rightarrow b, a c \rightarrow d \}$

计算  $\{ b, c \}_F^+ = \{ b, c \}$

$\because d \notin \{ b, c \}_F^+$

$\therefore$  不能去掉  $b c \rightarrow d$

❑ **Example 1:**  $F = \{ a \rightarrow b, b c \rightarrow d, a c \rightarrow d \}$

Give the minimal cover  $M$  for the set  $F$  of FDs.

❑ **Step 2:**

3) 假设去掉  $a c \rightarrow d$ , 则  $F = \{ a \rightarrow b, b c \rightarrow d \}$

计算  $\{ a, c \}_F^+ = \{ a, c, b, d \}$

$\therefore d \in \{ a, c \}_F^+$

$\therefore a c \rightarrow d$  是一个冗余的函数依赖关系, 可以从  $F$  中删除, 则  $F$  变为:

$F = \{ a \rightarrow b, b c \rightarrow d \}$

□  $F = \{ a \rightarrow b, b c \rightarrow d \}$

□ **Step 3:** 只需要考虑对  $b c \rightarrow d$  的处理

1) 假设将  $b c \rightarrow d$  精简为  $c \rightarrow d$ ，则将  $F$  转变为下面的函数依赖集： $G = \{ a \rightarrow b, c \rightarrow d \}$

计算  $\{ c \}_F^+ = \{ c \}$

$\because d \notin \{ c \}_F^+$

$\therefore$  不能用  $c \rightarrow d$  来代替  $b c \rightarrow d$

2) 假设将  $b c \rightarrow d$  精简为  $b \rightarrow d$ ，则将  $F$  转变为下面的函数依赖集： $G = \{ a \rightarrow b, b \rightarrow d \}$

计算  $\{ b \}_F^+ = \{ b \}$

$\because d \notin \{ b \}_F^+$

$\therefore$  也不能用  $b \rightarrow d$  来代替  $b c \rightarrow d$

- ❑ **Example 1:**  $F = \{ a \rightarrow b, b c \rightarrow d, a c \rightarrow d \}$   
Give the minimal cover  $M$  for the set  $F$  of FDs.

- ❑ **Step 3 & 4:**

计算结果为:  $F = \{ a \rightarrow b, b c \rightarrow d \}$